format-version: 1.2
date: 27:07:2016 15:10
saved-by: pgaudet
auto-generated-by: OBO-Edit 2.1.1-beta6
default-namespace: ME

[Term]
id: ME:0000001
name: modification effect
def: "Ontology that describes changes on function, property, localization, etc., following a modification (PTM, variation, etc)." [NP:PG]
created_by: pgaudet
creation_date: 2016-07-27T03:01:06Z

[Term]
id: ME:0000002
name: impact
def: "Relation that indicates that the modification causes a change on an observed parameter." [NP:PG]
is_a: ME:0000001 ! modification effect
created_by: pgaudet
creation_date: 2016-07-27T03:03:44Z

[Term]
id: ME:0000003
name: no impact
def: "Relation that indicates that the modification does not cause a change on an observed parameter." [NP:PG]
is_a: ME:0000001 ! modification effect
created_by: pgaudet
creation_date: 2016-07-27T03:04:59Z

[Term]
id: ME:0000004
name: decrease
def: "Relation that indicates that the modification causes a change on an observed parameter, by which the parameter is less important than that observed for the control." [NP:PG]
is_a: ME:0000002 ! impact
created_by: pgaudet
creation_date: 2016-07-27T03:05:41Z

[Term]
id: ME:0000005
name: increase
def: "Relation that indicates that the modification causes a change on an observed parameter, by which the parameter is more important or of higher amplitude than that observed for the control." [NP:PG]
is_a: ME:0000002 ! impact
created_by: pgaudet
creation_date: 2016-07-27T03:07:07Z

[Term]
id: ME:0000006
name: gain
def: "Relation that indicates that the modification causes a change on an observed parameter, which was not present in the control." [NP:PG]
is_a: ME:0000002 ! impact
created_by: pgaudet
creation_date: 2016-07-27T03:07:43Z
